src/Array.v
@@ -2125,8 +2125,8 @@ Theorem arrayN_list_eq : forall A (vs1 vs2 : list A) s m,
   arrayN s vs1 m -> arrayN s vs2 m -> vs1 = vs2.
 Proof.
   induction vs1; destruct vs2; simpl; intros; auto.
-  apply ptsto_valid in H0; congruence.
-  apply ptsto_valid in H; congruence.
+  apply ptsto_valid in H0; unfold emp in *; congruence.
+  apply ptsto_valid in H; unfold emp in *; congruence.
   apply ptsto_valid in H as Hx.
   apply ptsto_valid in H0 as Hy.
   rewrite Hx in Hy; inversion Hy; subst; clear Hx Hy; f_equal.
